realize.lisp
@@ -1,0 +1,73 @@
+
+
+(defun realize-at-1d (e id ctx)
+  (declare (xargs :guard (and (natp id)
+                              (halide-1dp e)
+                              (contextp ctx))))
+  (let* ((dim0 (car (halide-dims e)))
+         (rhs (halide-expr e))
+         (new-ctx (put-assoc dim0 id ctx)))
+    (ifix (expr-eval rhs new-ctx))))
+
+(assert-event (equal 3
+                     (realize-at-1d (cons '(f x)
+                                          '(+ x (* x 2)))
+                                    1 nil)))
+
+(assert-event (equal 63
+                     (realize-at-1d (cons '(f x)
+                                          '(* x (+ x 2)))
+                                    7 nil)))
+
+(assert-event (equal 5
+                     (realize-at-1d (cons '(f x)
+                                          '([] input x))
+                                    4
+                                    (cons '(input 1 1 2 3 5 8 13)
+                                          nil)
+                                    )))
+
+(defthm realize-type-correct
+  (implies (and (halidep e)
+                (natp i)
+                (contextp ctx))
+           (integerp (realize-at-1d e i ctx))))
+
+(defun realize-1d-inner (e size id ctx)
+  (declare (xargs :guard (and (halide-1dp e)
+                              (natp size)
+                              (natp id)
+                              (contextp ctx))))
+  (if (zp size)
+      nil
+    (cons (realize-at-1d e id ctx)
+          (realize-1d-inner e (1- size) (1+ id) ctx))))
+
+(defun realize-1d (e size ctx)
+  (declare (xargs :guard (and (halide-1dp e)
+                              (natp size)
+                              (contextp ctx))))
+  (realize-1d-inner e size 0 ctx))
+
+(defun induct-risz (n)
+  (if (zp n)
+      0
+    (1+ (induct-risz (1- n)))))
+
+(defthm realize-inner-size-good
+  (implies (and (halide-1dp e)
+                (natp N)
+                (natp i)
+                (contextp ctx))
+           (equal (len (realize-1d-inner e N i ctx))
+                  N))
+  :hints (("Goal"
+           :induct (induct-risz N)))
+  )
+
+(defthm realize-size-good
+  (implies (and (halide-1dp e)
+                (natp N)
+                (contextp ctx))
+           (equal (len (realize-1d e N ctx))
+                  N)))
